feat(relaxed): causal consistency & minor fixes of seq_cst

theories/concur/relaxed.v
@@ -16,7 +16,7 @@ Local Open Scope ident_scope.
 Local Open Scope lposet_scope.
 Local Open Scope pomset_scope.
 
-Module Export Lab.
+Module Lab.
 
 Module Lab.
 Section ClassDef.
@@ -76,6 +76,20 @@ End Lab.
 
 Export Lab.Exports.
 
+Variant typ := Read | Write | Undef.
+
+Definition eq_typ : rel typ := 
+  fun t1 t2 => match t1, t2 with
+  | Read , Read  => true
+  | Write, Write => true
+  | Undef, Undef => true
+  | _ , _        => false
+  end.
+
+Lemma eq_typP : Equality.axiom eq_typ.
+Proof. by case; case; constructor. Qed.
+
+Module Export Def.
 Section Def.
 Context {L : labType}.
 Implicit Types (l : L).
@@ -87,12 +101,24 @@ Definition com : rel L := Lab.com (Lab.class L).
 Definition is_write : pred L := Lab.is_write (Lab.class L).
 Definition is_read  : pred L := Lab.is_read  (Lab.class L).
 
+Canonical typ_eqMixin := EqMixin eq_typP.
+Canonical typ_eqType  := Eval hnf in EqType typ typ_eqMixin.
+
+Definition lab_typ l : typ := 
+  if is_read l then 
+    Read 
+  else if is_write l then 
+    Write
+  else Undef.
+
+End Def.
 End Def.
 
 Module Export Syntax.
 Notation "l1 '\>>' l2" := (com l1 l2) (at level 90).
 End Syntax.
 
+Module Export Theory.
 Section Theory.
 Context (L : labType).
 Implicit Types (l r w: L).
@@ -114,15 +140,33 @@ Lemma bot_nread :
 Proof. by case L=> ? [? []]. Qed.
 
 End Theory.
+End Theory.
 
 End Lab.
 
+Export Lab.Lab.Exports.
+Export Lab.Def.
+Export Lab.Syntax.
+Export Lab.Theory.
+
+
 Module Export ThrdPomset.
+
+Notation thrd_pomset E L Tid := 
+  (@pomset E _ (\i0 : Tid, bot : L)).
+
+Notation thrd_pomlang E L Tid := 
+  (@pomset E _ (\i0 : Tid, bot : L) -> Prop).
 
 Section Def.
 Context {E : identType} {L : labType}.
 Context {Tid : identType}.
-Implicit Types (p q : @pomset E _ (\i0 : Tid, bot : L)).
+(* data-type semantics *)
+Context (DS : ltsType L).
+(* thread semantics *)
+Context (TS : ltsType L).
+Implicit Types (d : DS) (s : TS).
+Implicit Types (p q : @thrd_pomset E L Tid).
 
 Definition fs_tid p e := 
   fst (fs_lab p e).
@@ -133,40 +177,16 @@ Definition fs_dlab p e :=
 Definition dlab_defined p := 
   [forall e : finsupp p, fs_dlab p (val e) != bot].
 
-Structure thrd_pomset : Type := ThrdPomset {
-  thrd_pomset_val :> @pomset E _ (\i0 : Tid, bot : L); 
-  _ : let p := thrd_pomset_val in 
-      dlab_defined p
-}.
+Definition lab_prj : Tid * L -> L := snd.
 
-Canonical thrd_pomset_subType := Eval hnf in [subType for thrd_pomset_val].
+Definition lts_thrd_pomlang d : thrd_pomlang E L Tid := 
+  fun p => (lts_pomlang d : pomlang E L bot) (Pomset.relabel lab_prj p).
+
+Lemma lab_prj_bot :
+  lab_prj (\i0, bot) = bot.
+Proof. done. Qed.
 
 End Def.
-
-Arguments thrd_pomset E L Tid : clear implicits.
-
-Section Instances. 
-
-Definition thrd_pomset_eqMixin E L Tid := 
-  Eval hnf in [eqMixin of (thrd_pomset E L Tid) by <:].
-Canonical thrd_pomset_eqType E L Tid := 
-  Eval hnf in EqType (thrd_pomset E L Tid) (@thrd_pomset_eqMixin E L Tid).
-
-Definition thrd_pomset_choiceMixin E L Tid :=
-  Eval hnf in [choiceMixin of (thrd_pomset E L Tid) by <:].
-Canonical thrd_pomset_choiceType E L Tid :=
-  Eval hnf in ChoiceType (thrd_pomset E L Tid) 
-                         (@thrd_pomset_choiceMixin E L Tid).
-
-(* Definition thrd_pomset_countMixin E L Tid := *)
-(*   Eval hnf in [countMixin of (@thrd_pomset E L Tid) by <:]. *)
-(* Canonical thrd_pomset_countType E L Tid := *)
-(*   Eval hnf in CountType (thrd_pomset E L Tid) (@thrd_pomset_countType E L Tid). *)
-
-(* Canonical thrd_pomset_subCountType E L Tid := *)
-(*   Eval hnf in [subCountType of (thrd_pomset E L Tid)]. *)
-
-End Instances.
 
 End ThrdPomset.
 
@@ -177,31 +197,25 @@ Context {Tid : identType}.
 Context (TS : ltsType L).
 Implicit Types (p q : @thrd_pomset E L Tid).
 
-Definition eqtid p : rel [Event of p] := 
+Definition eq_tid p : rel E := 
   fun e1 e2 => fs_tid p e1 == fs_tid p e2.
 
-Arguments eqtid p : clear implicits. 
+Arguments eq_tid p : clear implicits. 
 
-Lemma eqtid_refl p : reflexive (eqtid p).
-Proof. by rewrite /eqtid. Qed.
+Lemma eqtid_refl p : reflexive (eq_tid p).
+Proof. by rewrite /eq_tid. Qed.
 
-Lemma eqtid_sym p : symmetric (eqtid p).
-Proof. by rewrite /eqtid. Qed.
+Lemma eqtid_sym p : symmetric (eq_tid p).
+Proof. by rewrite /eq_tid. Qed.
 
-Lemma eqtid_trans p : transitive (eqtid p).
-Proof. by rewrite /eqtid=> ??? /eqP-> /eqP->. Qed.
+Lemma eqtid_trans p : transitive (eq_tid p).
+Proof. by rewrite /eq_tid=> ??? /eqP-> /eqP->. Qed.
 
-Definition lab_prj : Tid * L -> L := snd.
-
-Lemma lab_prj_bot :
-  lab_prj (\i0, bot) = bot.
-Proof. done. Qed.
-
-Definition po p := 
-  let q := Pomset.inter_rel (eqtid p) (@eqtid_refl p) (@eqtid_trans p) p in
-  Pomset.relabel lab_prj p lab_prj_bot (valP p). 
+Definition po p : thrd_pomset E L Tid := 
+  Pomset.inter_rel (eq_tid p) (@eqtid_refl p) (@eqtid_trans p) p.
 
 End ProgramOrder.
+
 
 Section SeqCst.
 Context {E : identType} {L : labType}.
@@ -215,6 +229,67 @@ Implicit Types (d : DS) (s : TS).
 Implicit Types (p q : @thrd_pomset E L Tid).
 
 Definition seq_cst d p := 
-  eq (po p) \supports (lts_pomlang d).
+  eq (po p) \supports (lts_thrd_pomlang d).
 
 End SeqCst.
+
+(* TODO: better name? *)
+Section ValueRelab. 
+Context {E : identType} {L : labType}.
+Context {Tid : identType}.
+(* data-type semantics *)
+Context (DS : ltsType L).
+(* thread semantics *)
+Context (TS : ltsType L).
+Implicit Types (p : @thrd_pomset E L Tid).
+
+(* checks that f is a value-relabeling of pomset p w.r.t. set of events es *)
+Definition is_val_relab p (es : {fset E}) (f : Tid * L -> L) := 
+  let lab e  := fs_lab  p (val e) in
+  let dlab e := fs_dlab p (val e) in
+  [&& (* labels of all events in es are preserved *)
+      [forall e : finsupp p, (val e \in es) ==> (f (lab e) == dlab e)]
+      (* types of all events are preserved (i.e. reads/writes are preserved) *)
+    & [forall e : finsupp p, lab_typ (f (lab e)) == lab_typ (dlab e)]
+  ].
+
+End ValueRelab. 
+
+
+Section CausalCst. 
+Context {E : identType} {L : labType}.
+Context {Tid : identType}.
+(* data-type semantics *)
+Context (DS : ltsType L).
+(* thread semantics *)
+Context (TS : ltsType L).
+
+Implicit Types (d : DS) (s : TS).
+Implicit Types (p : @thrd_pomset E L Tid).
+
+(* Causally relabeled threaded pomset language w.r.t. pomset language Q.
+ * Pomset p belongs to this language if: 
+ * (1) there exists maximal element e of p;
+ * (2) p is relabeling of some q \in Q such that this relabeling
+ *   (2.1) preserves labels of all events from the thread of e 
+ *         and all writes events (i.e. non-reads);
+ *   (2.2) preserves types (i.e. reads/writes) of all events.
+ *)
+Definition causal_relab (Q : pomlang E L bot) : thrd_pomlang E L Tid := 
+  fun p => exists f, exists q, exists e,
+    let es := 
+      [fset e' in finsupp p | eq_tid p e e' || ~~ is_read (fs_dlab p e)] 
+    in
+    [/\ is_val_relab p es f
+      , e \in finsupp p, lfsp_is_max p e
+      , Q q & q = Pomset.relabel f p
+    ].
+
+Definition causal d p := 
+  (pideal_lang p) \supports (causal_relab (lts_pomlang d)).
+
+Definition causal_cst d p := 
+  eq (po p) \supports (causal d).  
+
+End CausalCst.
+
